

$$\overrightarrow{a} = 
\begin{pmatrix}
	x - 2y \\
	2x - y \\
	2z
\end{pmatrix} ; \overrightarrow{b} = 
\begin{pmatrix}
	2 \\
	-2 \\
	1
\end{pmatrix}$$

if $\overrightarrow{a} = \overrightarrow{b}$, then,

$$\begin{pmatrix}
	x - 2y \\
	2x - y \\
	2z
\end{pmatrix} = \begin{pmatrix}
	2 \\
	-2 \\
	1
\end{pmatrix}$$

Converting this in matrix notation we have,

$$\begin{bmatrix}
1 & -2 & 0 \\
2 & -1 & 0 \\
0 & 0 & 2 
\end{bmatrix} = \begin{bmatrix}
2 \\
-2 \\
1
\end{bmatrix}$$

By Row Elimination we have,

$$\begin{bmatrix}
1 & -2 & 0 \\
0 & 3 & 0 \\
0 & 0 & 2 
\end{bmatrix} = \begin{bmatrix}
2 \\
-6 \\
1
\end{bmatrix}$$

Therefore by back-substitution we have,

$$\{z = \frac{1}{2}; y = -2; x = -2\} \in \mathbb{R}$$

