

$$\overrightarrow{a} = \begin{pmatrix}
-1 \\
2 \\
3
\end{pmatrix}, \overrightarrow{b} = \begin{pmatrix}
2 \\
-2 \\
0
\end{pmatrix}, \overrightarrow{c} = \begin{pmatrix}
3 \\
0 \\
-1
\end{pmatrix}; a \in \mathbb{R}$$

i) $2\overrightarrow{a} - \overrightarrow{b} + 5\overrightarrow{c}$

$$2\overrightarrow{a} - \overrightarrow{b} + 5\overrightarrow{c} = \begin{pmatrix}
-2 \\
4 \\
6
\end{pmatrix} - \begin{pmatrix}
2 \\
-2 \\
0
\end{pmatrix} + \begin{pmatrix}
15 \\
0 \\
-5
\end{pmatrix} = \begin{pmatrix}
11 \\
6 \\
1
\end{pmatrix}$$

ii) $4\overrightarrow{a} + \alpha\overrightarrow{b} - 2\overrightarrow{c}$

$$4\overrightarrow{a} + \alpha\overrightarrow{b} - 2\overrightarrow{c} = \begin{pmatrix}
-4 \\
8 \\
12
\end{pmatrix} + \alpha\begin{pmatrix}
2 \\
-2 \\
0
\end{pmatrix} + \begin{pmatrix}
-6 \\
0 \\
2
\end{pmatrix} = \begin{pmatrix}
-10 + 2\alpha \\
8 - 2\alpha \\
14
\end{pmatrix}

