

$$\overrightarrow{u} = \begin{pmatrix}
1 \\
-1 \\
0 \\
2
\end{pmatrix}; \overrightarrow{v} = \begin{pmatrix}
-2 \\
-1 \\
1 \\
-4
\end{pmatrix} \& \overrightarrow{w} = \begin{pmatrix}
3 \\
2 \\
-1 \\
0
\end{pmatrix}$$

a) $\overrightarrow{a} \in \mathbb{R} : 2\overrightarrow{u} - 3\overrightarrow{v} - \overrightarrow{a} = \overrightarrow{w}$

$$\therefore \begin{pmatrix}
2 \\
-2 \\
0 \\
4
\end{pmatrix} + \begin{pmatrix}
6 \\
3 \\
-3 \\
12
\end{pmatrix} - \begin{pmatrix}
3 \\
2 \\
-1 \\
0
\end{pmatrix} = \overrightarrow{a}$$

$$\implies \overrightarrow{a} = \begin{pmatrix}
11 \\
3 \\
-4 \\
16
\end{pmatrix}$$

